inprogress

theories/Hoare.v
@@ -2,10 +2,9 @@
 
 This file formalizes Hoare Logic:
 
-- heap entailement, written [H ==> H'],
 - definition of Hoare triple (total correctness)
-- consequence rule
-- rule for term constructs.
+- structural rules for Hoare triples
+- reasoning rule for term constructs.
 
 It does not include reasoning rules for primitive operations on the heap,
 because these are more naturally expressed directly in Separation Logic.
@@ -20,115 +19,18 @@ From Sep Require Export Semantics.
 Open Scope fmap_scope.
 
 
+
 (* ********************************************************************** *)
-(** * Entailment *)
+(** * Definition of Hoare triples *)
 
-(** The definition of entailment is polymorphic in the type of heaps,
-    which could be state, but also more elaborated structures in
-    extensions of Separation Logic (e.g. with time credits). *)
+Definition hoare (t:trm) (H:state->Prop) (Q:val->state->Prop) :=
+  forall h, H h -> exists h' v, eval h t h' v /\ Q v h'.
 
-
-(* ---------------------------------------------------------------------- *)
-(* ** Predicate extensionality, specialized to heap predicates *)
-
-(** Predicate extensionality follows from functional extensional
-    and propositional extensionality, which we take as axiom
-    (in TLC's LibAxioms file). *)
-
-Lemma hprop_extens : forall A (H1 H2:A->Prop),
-  (forall h, H1 h <-> H2 h) ->
-  (H1 = H2).
-Proof using.
-  introv M. applys fun_ext_1. intros h. applys* prop_ext.
-Qed.
-
-(* ---------------------------------------------------------------------- *)
-(* ** Definition of entailment *)
-
-(** [H1 ==> H2] is defined as [forall h, H1 h -> H2 h]. *)
-
-Definition himpl A (H1 H2:A->Prop) :=
-  forall x, H1 x -> H2 x.
-
-Notation "H1 ==> H2" := (himpl H1 H2)
-  (at level 55) : heap_scope.
-
-(** [Q1 ===> Q2] is defined as [forall x h, Q1 x h -> Q2 x h].
-    It is thus equivalent to [forall x, Q1 x ==> Q2 x].
-    Thus, invoking [intro] on a [===>] goal leaves a [==>] goal. *)
-
-Definition qimpl A B (Q1 Q2:A->B->Prop) :=
-  forall r, himpl (Q1 r) (Q2 r).
-
-Notation "Q1 ===> Q2" := (qimpl Q1 Q2)
-  (at level 55) : heap_scope.
-
-Open Scope heap_scope.
-
-
-(* ---------------------------------------------------------------------- *)
-(* ** Properties of entailment *)
-
-Section HimplProp.
-Variable A : Type.
-Implicit Types H : A -> Prop.
-
-Hint Unfold himpl.
-
-(** Entailment is reflexive, symmetric, transitive *)
-
-Lemma himpl_refl : forall H,
-  H ==> H.
-Proof using. intros h. auto. Qed.
-
-Lemma himpl_trans : forall H2 H1 H3,
-  (H1 ==> H2) ->
-  (H2 ==> H3) ->
-  (H1 ==> H3).
-Proof using. introv M1 M2. intros h H1h. eauto. Qed.
-
-Lemma himpl_antisym : forall H1 H2,
-  (H1 ==> H2) ->
-  (H2 ==> H1) ->
-  (H1 = H2).
-Proof using. introv M1 M2. applys pred_ext_1. intros h. iff*. Qed.
-
-(** Paragraphe of the definition, used by tactics *)
-
-Lemma himpl_inv : forall H1 H2 (h:A),
-  (H1 ==> H2) ->
-  (H1 h) ->
-  (H2 h).
-Proof using. auto. Qed.
-
-(** Reformulation of reflexivity, used by tactics *)
-
-Lemma himpl_of_eq : forall H1 H2,
-  H1 = H2 ->
-  H1 ==> H2.
-Proof. intros. subst. applys~ himpl_refl. Qed.
-
-Lemma himpl_of_eq_sym : forall H1 H2,
-  H1 = H2 ->
-  H2 ==> H1.
-Proof. intros. subst. applys~ himpl_refl. Qed.
-
-End HimplProp.
-
-Arguments himpl_of_eq [A] [H1] [H2].
-Arguments himpl_of_eq_sym [A] [H1] [H2].
-Arguments himpl_antisym [A] [H1] [H2].
-
-Hint Resolve himpl_refl.
-
-(** Reflexivity for postconditions *)
-
-Lemma qimpl_refl : forall A B (Q:A->B->Prop),
-  Q ===> Q.
-Proof using. intros. hnfs*. Qed.
-
-Hint Resolve qimpl_refl.
-
+Implicit Types H : state->Prop.
+Implicit Types f : bind.
+Implicit Types v w : val.
+Implicit Types t : trm.
+Implicit Types vs : vals.
 
 (* ---------------------------------------------------------------------- *)
 (* ** Tactic [himpl_fold] *)
@@ -145,19 +47,6 @@ Ltac himpl_fold_core tt :=
 Tactic Notation "himpl_fold" := himpl_fold_core tt.
 Tactic Notation "himpl_fold" "~" := himpl_fold; auto_tilde.
 Tactic Notation "himpl_fold" "*" := himpl_fold; auto_star.
-
-
-(* ********************************************************************** *)
-(** * Definition of Hoare triples *)
-
-Definition hoare (t:trm) (H:state->Prop) (Q:val->state->Prop) :=
-  forall h, H h -> exists h' v, eval h t h' v /\ Q v h'.
-
-Implicit Types H : state->Prop.
-Implicit Types f : bind.
-Implicit Types v w : val.
-Implicit Types t : trm.
-Implicit Types vs : vals.
 
 
 (* ********************************************************************** *)
