theories/SLFDirect.v
@@ -1,0 +1,21 @@
+(**
+
+Separation Logic Foundations
+
+Chapter: "Himpl".
+
+Author: Arthur Charguéraud.
+License: MIT.
+
+*)
+
+Set Implicit Arguments.
+From Sep Require Export SLFHprop.
+From Sep Require SepBase.
+
+(** Implicit Types *)
+
+Implicit Types H : hprop.
+Implicit Types Q : val->hprop.
+
+
